theories/heap_lang/lib/atomic_snapshot_spec.v
@@ -3,7 +3,7 @@ From iris.heap_lang Require Export lifting notation.
 From iris.base_logic.lib Require Export invariants.
 From iris.program_logic Require Export atomic.
 From iris.proofmode Require Import tactics.
-From iris.heap_lang Require Import proofmode notation par prophecy.
+From iris.heap_lang Require Import proofmode notation par.
 From iris.bi.lib Require Import fractional.
 Set Default Proof Using "Type".
 
