theories/heap_lang/lib/coin_flip.v
@@ -4,7 +4,6 @@ From iris.program_logic Require Export atomic.
 From iris.proofmode Require Import tactics.
 From iris.heap_lang Require Import proofmode notation par.
 From iris.bi.lib Require Import fractional.
-From iris.heap_lang Require Import prophecy.
 Set Default Proof Using "Type".
 
 (** Nondeterminism and Speculation:
@@ -29,19 +28,19 @@ Section coinflip.
     λ: "x",
     "x" <- #0 ;;
      rand #().
-    
+
   Context `{!heapG Σ} (N: namespace).
-  
+
   Lemma rand_spec :
     {{{ True }}} rand #() {{{ (b : bool), RET #b; True }}}.
   Proof using N.
     iIntros (Φ) "_ HP".
     wp_lam. wp_alloc l as "Hl". wp_lam.
     iMod (inv_alloc N _ (∃ (b: bool), l ↦ #b)%I with "[Hl]") as "#Hinv"; first by eauto.
-    wp_apply wp_fork. iSplitL.
+    wp_apply wp_fork.
+    - iInv N as (b) ">Hl". wp_store. iModIntro. iSplitL; eauto.
     - wp_lam. iInv N as (b) ">Hl". wp_load. iModIntro. iSplitL "Hl"; first by eauto.
       iApply "HP". done.
-    - iInv N as (b) ">Hl". wp_store. iModIntro. iSplitL; eauto.    
   Qed.
 
   Lemma earlyChoice_spec (x: loc) :
@@ -50,7 +49,7 @@ Section coinflip.
         @ ⊤
     <<< ∃ (b: bool), x ↦ #0, RET #b >>>.
   Proof using N.
-    iApply wp_atomic_intro. iIntros (Φ) "AU". wp_lam.    
+    iApply wp_atomic_intro. iIntros (Φ) "AU". wp_lam.
     wp_bind (rand _)%E. iApply rand_spec; first done.
     iIntros (b) "!> _". wp_let.
     wp_bind (_ <- _)%E.
@@ -78,47 +77,48 @@ Section coinflip.
     iMod ("Hclose" $! true with "[Hl]") as "AU"; first by eauto.
     iModIntro. wp_seq.
     iApply rand_spec; first done.
-    iIntros (b) "!> _".    
+    iIntros (b) "!> _".
     Abort.
 
 End coinflip.
 
-Section coinflip_with_prophecy.  
-    
-  Context `{!heapG Σ} `{pr: prophecy} (N: namespace).
+Section coinflip_with_prophecy.
+
+  Context `{!heapG Σ} (N: namespace).
 
   Definition val_to_bool v : bool :=
     match v with
-    | LitV (LitBool b) => b
-    | _                => true
+    | Some (LitV (LitBool b)) => b
+    | _                       => true
     end.
 
   Definition lateChoice_proph: val :=
     λ: "x",
-      let: "p" := new_prophecy pr #() in
+      let: "p" := new prophecy in
       "x" <- #0 ;;
       let: "r" := rand #() in
-      resolve_prophecy pr "p" "r".
-  
+      resolve "p" to "r" ;;
+      "r".
+
   Lemma lateChoice_proph_spec (x: loc) :
     <<< x ↦ - >>>
         lateChoice_proph #x
         @ ⊤
-    <<< ∃ (b: bool), x ↦ #0, RET #b >>>. 
+    <<< ∃ (b: bool), x ↦ #0, RET #b >>>.
   Proof using N.
     iApply wp_atomic_intro. iIntros (Φ) "AU". wp_lam.
-    wp_apply new_prophecy_spec; first done.
+    wp_apply wp_new_proph; first done.
     iIntros (p) "Hp". iDestruct "Hp" as (v) "Hp".
-    wp_let.    
+    wp_let.
     wp_bind (_ <- _)%E.
     iMod "AU" as "[Hl [_ Hclose]]".
     iDestruct "Hl" as (v') "Hl".
     wp_store.
     iMod ("Hclose" $! (val_to_bool v) with "[Hl]") as "HΦ"; first by eauto.
     iModIntro. wp_seq. wp_apply rand_spec; try done.
-    iIntros (b') "_". wp_let.
-    iApply (resolve_prophecy_spec with "Hp").
-    iNext. iIntros (->). done.
+    iIntros (b') "_". wp_let. wp_bind (resolve _ to _)%E.
+    iApply (wp_resolve_proph with "Hp").
+    iNext. iIntros (->). wp_seq. done.
   Qed.
 
 End coinflip_with_prophecy.
